theories/micromega/ZifyBool.v
@@ -14,7 +14,8 @@ Local Open Scope Z_scope.
 (* Instances of [ZifyClasses] for dealing with boolean operators. *)
 
 Instance Inj_bool_bool : InjTyp bool bool :=
-  { inj := (fun x => x) ; pred := (fun x => True) ; cstr := (fun _ => I)}.
+  { inj := (fun x => x) ; pred := (fun b => b = true \/ b = false) ;
+    cstr := (ltac:(intro b; destruct b; tauto))}.
 Add InjTyp Inj_bool_bool.
 
 (** Boolean operators *)
@@ -45,6 +46,10 @@ Instance Op_xorb : BinOp xorb :=
     TBOpInj := xorb_eq }.
 Add BinOp Op_xorb.
 
+Instance Op_eqb : BinOp eqb :=
+  { TBOp := eqb; TBOpInj := ltac:(reflexivity) }.
+Add BinOp Op_eqb.
+
 Instance Op_negb : UnOp negb :=
   { TUOp := negb ; TUOpInj := ltac:(reflexivity)}.
 Add UnOp Op_negb.
@@ -65,6 +70,7 @@ Add CstOp Op_false.
 
 Instance Op_Zeqb : BinOp Z.eqb :=
   { TBOp := Z.eqb ; TBOpInj := ltac:(reflexivity)}.
+Add BinOp Op_Zeqb.
 
 Instance Op_Zleb : BinOp Z.leb :=
   { TBOp := Z.leb;
@@ -82,6 +88,7 @@ Instance Op_Zltb : BinOp Z.ltb :=
   { TBOp := Z.ltb ;
     TBOpInj := ltac:(reflexivity)
   }.
+Add BinOp Op_Zltb.
 
 Instance Op_Zgtb : BinOp Z.gtb :=
   { TBOp := Z.gtb;
@@ -137,3 +144,38 @@ Instance Op_nat_ltb : BinOp Nat.ltb :=
     TBOpInj := Z_of_nat_ltb_iff
   }.
 Add BinOp Op_nat_ltb.
+
+Lemma b2n_b2z :  forall x,  Z.of_nat (Nat.b2n x) = Z.b2z x.
+Proof.
+  intro.
+  destruct x ; reflexivity.
+Qed.
+
+Instance Op_b2n : UnOp Nat.b2n :=
+  { TUOp := Z.b2z;
+    TUOpInj := b2n_b2z }.
+Add UnOp Op_b2n.
+
+Instance Op_b2z : UnOp Z.b2z :=
+  { TUOp := Z.b2z;
+    TUOpInj := ltac:(reflexivity) }.
+Add UnOp Op_b2z.
+
+Lemma b2z_spec : forall b, (b = true /\ Z.b2z b = 1) \/ (b = false /\ Z.b2z b = 0).
+Proof.
+  destruct b ; simpl; intuition congruence.
+Qed.
+
+Instance b2zSpec : UnOpSpec Z.b2z :=
+  {| UPred := fun b r => (b = true /\ r = 1) \/ (b = false /\ r = 0);
+     USpec := b2z_spec
+  |}.
+Add UnOpSpec b2zSpec.
+
+Ltac elim_bool_cstr :=
+  repeat match goal with
+         | C : ?B = true \/ ?B = false |- _ =>
+           destruct C ; subst
+         end.
+
+Ltac Zify.zify_post_hook ::= elim_bool_cstr.
